exercises_and_homework_day_4_teacher.v
@@ -1,0 +1,832 @@
+(** * Exploring equality via homotopy and proof assistants - Day 4 - Equality of types *)
+(** This file contains the exercises for Day 4.  Some are explicitly
+    marked as "Homework"; the rest can be done either in class or for
+    homework.
+
+    When doing exercises on your own, feel free to skip around; there
+    are some interesting puzzles near the bottom.
+
+    If you feel like you know exactly how a proof will go, but find it
+    painful and tedius to write out the proof terms explicitly, come
+    find me.  Coq has a lot of support for automation and taking care
+    of things that are easy and verbose, so you don't have to.
+    Proving should feel like a game.  If it doesn't, I can probably
+    help you with that.
+
+    This file is set up a bit differently from previous days; I want
+    you to generate more of the ideas for this one.  So I've left in
+    only the stubs at the top for you, without the comments that
+    pepper my version of the file.  You should follow along, copying
+    the the code as I reveal or type it on the screen, so you can play
+    with it to make suggestions.  I'll be releasing my (filled in)
+    version of the file after class today, so that you have the
+    comments for future reference. *)
+
+(** The following are placeholders; [admit] indicates that something
+    should be filled in later. *)
+
+Axiom admit : forall {T}, T.
+
+(** Some filled in exercises from yesterday; feel free to paste more here. *)
+
+Notation refl := eq_refl.
+Definition sym : forall A (x y : A), x = y -> y = x
+  := fun A x y p
+     => match p in (_ = y) return y = x with
+          | refl => refl
+        end.
+
+(** We allow writing [sym p] to mean [sym _ _ _ p] *)
+
+Arguments sym {A x y} p, A x y p.
+
+Definition trans : forall A (x y z : A), x = y -> y = z -> x = z
+  := fun A x y z p
+     => match p in (_ = y) return y = z -> x = z with
+          | refl => fun q => match q in (_ = z) return x = z with
+                               | refl => refl
+                             end
+        end.
+
+Arguments trans {A x y z} !p !q, A x y z !p !q.
+
+Definition ap : forall A B (f : A -> B) (x y : A), x = y -> f x = f y
+  := fun A B f x y p
+     => match p with
+          | refl => refl
+        end.
+
+Arguments ap {A B} f {x y} p, {A B} f x y p, A B f x y p.
+
+Definition J : forall {A} {x : A} (P : forall y, x = y -> Type),
+                 P x refl -> forall {y} (H : x = y), P y H
+  := fun A x P k y H
+     => match H with
+          | eq_refl => k
+        end.
+
+Definition sym_sym : forall A (x y : A) (p : x = y), sym (sym p) = p
+  := fun A x y p
+     => match p with
+          | refl => refl
+        end.
+
+Arguments sym_sym {A x y} p, A x y p.
+
+Definition ap_sym : forall {A B} (f : A -> B) {x y : A} (p : x = y),
+                         ap f (sym p) = sym (ap f p)
+  := fun A B f x y p
+     => match p with
+          | refl => refl
+        end.
+
+Arguments ap_sym {A B} f {x y} p, A B f x y p.
+
+Definition ap_trans : forall {A B} (f : A -> B) {x y z : A} (p : x = y) (q : y = z),
+                           ap f (trans p q) = trans (ap f p) (ap f q)
+  := fun A B f x y z p
+     => match p with
+          | refl => fun q => match q with
+                               | refl => refl
+                             end
+        end.
+
+Arguments ap_trans {A B} f {x y z} p q, A B f x y z p q.
+
+Definition ap_compose : forall {A B C} (f : A -> B) (g : B -> C) {x y : A} (p : x = y),
+                           ap g (ap f p) = ap (fun x => g (f x)) p
+  := fun A B C f g x y p
+     => match p with
+          | refl => refl
+        end.
+
+Arguments ap_trans {A B} f {x y z} p q, A B f x y z p q.
+
+Definition sym_trans : forall {A} {x y z : A} (p : x = y) (q : y = z),
+                           sym (trans p q) = trans (sym q) (sym p)
+  := fun A x y z p
+     => match p with
+          | refl => fun q => match q with
+                               | refl => refl
+                             end
+        end.
+
+Definition trans_1p : forall {A} {x y : A} (p : x = y), trans refl p = p
+  := fun A x y p
+     => match p with
+          | refl => refl
+        end.
+
+Definition trans_pp_p : forall {A} {x y z w : A} (p : x = y) (q : y = z) (r : z = w),
+                          trans (trans p q) r = trans p (trans q r)
+  := fun A x y z w p
+     => match p with
+          | refl => fun q => match q with
+                               | refl => fun r => match r with
+                                                    | refl => refl
+                                                  end
+                             end
+        end.
+
+Definition trans_p1 : forall {A} {x y : A} (p : x = y), trans p refl = p
+  := fun A x y p
+     => match p with
+          | refl => refl
+        end.
+
+Definition trans_Vp : forall {A} {x y : A} (p : x = y), trans (sym p) p = refl
+  := fun A x y p
+     => match p with
+          | refl => refl
+        end.
+
+Definition trans_pV : forall {A} {x y : A} (p : x = y), trans p (sym p) = refl
+  := fun A x y p
+     => match p with
+          | refl => refl
+        end.
+
+Definition concat_Ap
+: forall {A B} (f g : A -> B)
+         (T : forall x, f x = g x),
+    forall {x y : A} (m : x = y),
+      trans (ap f m) (T y) = trans (T x) (ap g m).
+Proof.
+  intros A B f g T x y m.
+  destruct m; simpl.
+  destruct (T x).
+  reflexivity.
+Defined.
+
+Definition concat_A1p
+: forall {A} (f : A -> A)
+         (T : forall x, f x = x),
+    forall {x y : A} (m : x = y),
+      trans (ap f m) (T y) = trans (T x) m.
+Proof.
+  intros A f T x y m.
+  destruct m; simpl.
+  destruct (T x).
+  reflexivity.
+Defined.
+
+Definition concat_Ap1
+: forall {A} (f : A -> A)
+         (T : forall x, x = f x),
+    forall {x y : A} (m : x = y),
+      trans m (T y) = trans (T x) (ap f m).
+Proof.
+  intros A f T x y m.
+  destruct m; simpl.
+  destruct (T x).
+  reflexivity.
+Defined.
+
+Definition function_code : forall {A B} (f g : forall a : A, B a), Type
+  := fun A B f g => forall a : A, f a = g a.
+
+Definition function_encode : forall {A B} {f g : forall a : A, B a}, f = g -> function_code f g
+  := fun A B f g H a
+     => match H with
+          | refl => refl
+        end.
+
+Definition function_encode_sym
+: forall {A B f g} (p : f = g) x,
+    sym (@function_encode A B f g p x) = function_encode (sym p) x
+  := fun A B f g p x
+     => match p with
+          | refl => refl
+        end.
+
+Definition function_encode_trans
+: forall {A B f g h} (p : f = g) (q : g = h) x,
+    trans (@function_encode A B f g p x)
+          (@function_encode A B g h q x)
+    = function_encode (trans p q) x
+  := fun A B f g h p
+     => match p with
+          | refl => fun q x => match q with
+                                 | refl => refl
+                               end
+        end.
+
+Definition function_encode_ap : forall {A B C} {f g : A -> B} (p : f = g) (f' : B -> C) x,
+                                   ap f' (@function_encode A (fun _ => B) f g p x)
+                                   = function_encode (ap (fun f'' x' => f' (f'' x')) p) x
+  := fun A B C f g p f' x
+     => match p with
+          | refl => refl
+        end.
+
+Notation sig := sigT.
+Notation exist := existT.
+Notation "{ x  |  P }" := ({ x : _ & P }) : type_scope.
+Notation "{ x : A  |  P }" := ({ x : A & P }) : type_scope.
+Notation "( x ; p )" := (existT _ x p).
+Notation "x .1" := (projT1 x) (at level 3, format "x '.1'").
+Notation "x .2" := (projT2 x) (at level 3, format "x '.2'").
+
+Definition sigma_code : forall {A B} (x y : { a : A | B a }), Type
+  := fun A B x y
+     => { p : x.1 = y.1 | J (fun a _ => B a) x.2 p = y.2 }.
+
+Definition sigma_encode : forall {A B} {x y : { a : A | B a }}, x = y -> sigma_code x y
+  := fun A B x y p
+     => match p with
+          | refl => (refl; refl)
+        end.
+
+Definition sigma_decode : forall {A B} {x y : { a : A | B a }}, sigma_code x y -> x = y.
+Proof.
+  refine (fun A B x y
+          => match x, y return sigma_code x y -> x = y with
+               | (x1; x2), (y1; y2)
+                 => fun p => _
+             end).
+  destruct p as [p q].
+  simpl in *.
+  destruct q.
+  destruct p; simpl.
+  exact refl.
+Defined.
+
+Definition sigma_endecode : forall {A B} {x y : { a : A | B a }} (p : sigma_code x y),
+                             sigma_encode (sigma_decode p) = p.
+Proof.
+  intros A B x y p.
+  destruct x, y, p as [p q]; simpl in *.
+  destruct q, p; simpl.
+  reflexivity.
+Defined.
+
+Definition sigma_deencode : forall {A B} {x y : { a : A | B a }} (p : x = y),
+                             sigma_decode (sigma_encode p) = p.
+Proof.
+  intros A B x y p.
+  destruct p, x; simpl.
+  reflexivity.
+Defined.
+
+Definition is_prop : Type -> Type
+  := fun A => forall x y : A, x = y.
+
+(** We classify the equality type of propositions. *)
+
+Definition prop_code : forall {A} (allpaths : is_prop A) (x y : A), Type
+  := fun A allpaths x y => unit.
+
+Definition prop_encode : forall {A} (allpaths : is_prop A) {x y : A},
+                           x = y -> prop_code allpaths x y
+  := fun _ _ _ _ _ => tt.
+
+(** You can fill in the proof here from day 3 *)
+Definition prop_decode : forall {A} (allpaths : is_prop A) {x y : A},
+                           prop_code allpaths x y -> x = y
+  := admit.
+
+
+Definition prop_deencode : forall {A} (allpaths : is_prop A) {x y : A} (p : x = y),
+                             prop_decode allpaths (prop_encode allpaths p) = p
+  := admit.
+
+(** ** Equality of types *)
+
+(** *** Motivating Puzzle *)
+
+(** Puzzle for the day: classify the equalities of types.  That is,
+    fill in the following: *)
+
+Definition Type_code : forall (x y : Type), Type
+  := admit.
+
+Definition Type_encode : forall {x y : Type}, x = y -> Type_code x y
+  := admit.
+
+(** The following are unprovable in Coq, currently.  They are
+    collectively known as the "univalence axiom". *)
+
+Axiom Type_decode : forall {x y : Type}, Type_code x y -> x = y.
+Axiom Type_endecode : forall {x y : Type} (p : Type_code x y),
+                        Type_encode (Type_decode p) = p.
+Axiom Type_deencode : forall {x y : Type} (p : x = y),
+                        Type_decode (Type_encode p) = p.
+
+(** *** Provable equalities *)
+
+(** What equalities of types are provable? *)
+
+(** Ask the students to come up with this. *)
+
+
+
+
+
+
+
+
+
+
+
+
+
+
+
+
+
+
+
+
+
+
+
+
+
+
+
+
+
+
+
+
+
+
+
+
+Definition unit_refl : unit = unit
+  := admit.
+
+(** Can you prove this one?  (Take a minute to try on your own.) *)
+
+Inductive unit1 := tt1.
+Inductive unit2 := tt2.
+
+Definition unit12 : unit1 = unit2
+  := admit.
+
+(** Can you prove other ones? *)
+
+(** *** Provable inequalities *)
+
+(** What equalities of types are provably absurd? *)
+
+(** Ask the students to come up with this. *)
+
+
+
+
+
+
+
+
+
+
+
+
+
+
+
+
+
+
+
+
+
+
+
+
+
+Definition unit_Empty_set_absurd : unit = Empty_set -> Empty_set
+  := admit.
+
+(** More generally, when are two types provably different? *)
+
+
+
+
+
+
+
+
+
+
+
+
+
+
+
+
+
+
+
+
+
+
+
+
+
+
+
+
+
+
+
+
+
+
+
+
+
+
+(** *** Isomorphisms *)
+
+(** We can define a notion of isomorphism: *)
+
+Class IsIsomorphism {A B} (f : A -> B)
+  := { iso_inv : B -> A;
+       right_inv : forall x : B, f (iso_inv x) = x;
+       left_inv : forall x : A, iso_inv (f x) = x }.
+
+Arguments iso_inv {A B} f {_} _.
+Arguments right_inv {A B f _ _}, {A B} f {_} _.
+Arguments left_inv {A B f _ _}, {A B} f {_} _.
+
+Record Isomorphic A B
+  := { iso_fun : A -> B;
+       iso_isiso : IsIsomorphism iso_fun }.
+
+Arguments iso_fun {A B} _ _.
+
+(** Let us use an object of type [Isomorphic] as a function: *)
+
+Coercion iso_fun : Isomorphic >-> Funclass.
+
+(** Tell Coq that the function associated to an [Isomorphic] object is
+    always an isomorphism. *)
+
+Existing Instance iso_isiso.
+
+Notation "A <~=~> B" := (Isomorphic A B) (at level 70).
+Notation "A ≅ B" := (Isomorphic A B) (at level 70).
+
+(** We can prove the standard properties about isomorphisms: *)
+
+Definition Isomorphic_refl : forall {A}, A ≅ A
+  := fun A => {| iso_fun x := x;
+                 iso_isiso := {| iso_inv x := x;
+                                 right_inv x := refl : (fun x => x) x = x;
+                                 left_inv x := refl |} |}.
+
+Definition Isomorphic_inverse : forall {A B}, A ≅ B -> B ≅ A
+  := fun A B e =>
+       {| iso_fun := iso_inv e;
+          iso_isiso := {| iso_inv := iso_fun e;
+                          right_inv := left_inv e;
+                          left_inv := right_inv e |} |}.
+
+Definition Isomorphic_compose : forall {A B C}, A ≅ B -> B ≅ C -> A ≅ C
+  := fun A B C e1 e2 =>
+       {| iso_fun x := iso_fun e2 (iso_fun e1 x);
+          iso_isiso := {| iso_inv x := iso_inv e1 (iso_inv e2 x);
+                          right_inv x := trans (ap e2 (right_inv e1 (iso_inv e2 x)))
+                                               (right_inv e2 x);
+                          left_inv x := trans (ap (iso_inv e1) (left_inv e2 (e1 x)))
+                                              (left_inv e1 x) |} |}.
+
+(** We would like to prove the last corresponding law: *)
+
+Definition Isomorphic_ap : forall (f : Type -> Type) {A B}, A ≅ B -> f A ≅ f B
+  := admit.
+
+(** But it's not provable!  Here's a counter-example: *)
+
+(** Recall the taboo from earlier; we can't prove equality of two
+    identical types defined separately.  But if we could prove
+    [Isomorphic_ap], then we could prove this! *)
+
+Definition iso_unit2_unit1 : unit2 ≅ unit1
+  := admit.
+
+Definition taboo1 : unit1 = unit2 :> Type
+  := Isomorphic_ap (fun T => T = unit2) iso_unit2_unit1 refl.
+
+(** Ooops!  We'll be coming back to this soon. *)
+
+(** More practice: You can prove the higher groupoid laws about
+    isomorphisms, but it's a bit of a pain. *)
+
+(** Before dealing with the taboo above, let's classify the equality
+    space of isomorphisms. *)
+
+(** Recall the encode-decode method of yesterday: *)
+
+Definition unit_code : forall (x y : unit), Type
+  := fun _ _ => unit.
+
+(** We use curlie braces to not have to pass the [x] and [y] around
+    all the time. *)
+
+Definition unit_encode : forall {x y : unit}, x = y -> unit_code x y
+  := fun _ _ _ => tt.
+
+Definition unit_decode : forall {x y : unit}, unit_code x y -> x = y
+  := fun x y _
+     => match x, y with
+          | tt, tt => refl
+        end.
+
+Definition unit_endecode : forall {x y} (p : unit_code x y),
+                             unit_encode (unit_decode p) = p
+  := fun x y p
+     => match p with
+          | tt => refl
+        end.
+
+Definition unit_deencode : forall {x y} (p : x = y),
+                             unit_decode (unit_encode p) = p
+  := fun x y p
+     => match p with
+          | refl => match x with
+                      | tt => refl
+                    end
+        end.
+
+(** Let's add another piece to this puzzle, tying some more things together. *)
+
+(** Ask the students if anyone notices anything. *)
+
+Definition unit_iso : forall x y : unit, (x = y) ≅ unit
+  := fun x y
+     => {| iso_fun := unit_encode;
+           iso_isiso := {| iso_inv := unit_decode;
+                           right_inv := unit_endecode;
+                           left_inv := unit_deencode |} |}.
+
+(** Now, continuing on to isomorphisms... *)
+
+(** Let's assume functional extensionality; it's needed, here. *)
+
+Section assume_funext.
+  Context (function_decode : forall {A B} {f g : forall a : A, B a}, function_code f g -> f = g)
+          (function_endecode : forall {A B} {f g : forall a : A, B a} (p : function_code f g),
+                                 function_encode (function_decode p) = p)
+          (function_deencode : forall {A B} {f g : forall a : A, B a} (p : f = g),
+                                 function_decode (function_encode p) = p).
+
+  Definition iso_code : forall {A B} (x y : A ≅ B), Type
+    := admit.
+
+  Definition iso_encode : forall {A B} {x y : A ≅ B}, x = y -> iso_code x y
+    := admit.
+
+  Definition iso_decode : forall {A B} {x y : A ≅ B}, iso_code x y -> x = y
+    := admit.
+
+  Definition iso_endecode : forall {A B} {x y : A ≅ B} (p : iso_code x y),
+                              iso_encode (iso_decode p) = p
+    := admit.
+
+  Definition iso_deencode : forall {A B} {x y : A ≅ B} (p : x = y),
+                              iso_decode (iso_encode p) = p
+    := admit.
+
+  (** Ooops.  Turns out this isn't provable.  Challenge: Figure out why. *)
+
+End assume_funext.
+
+(** *** Equivalences *)
+
+(** We can define a slight variation on isomorphisms, called
+    "contractible fibers", which generalizes the notion of
+    injective+surjective.  If you're interested in the various ways of
+    formulating equivalences, Chapter 4 of the HoTT Book
+    (http://homotopytypetheory.org/book/) is an excellent resource. *)
+
+Class Contr (A : Type)
+  := { center : A;
+       contr : forall y, center = y }.
+
+Arguments center A {_}.
+
+Class IsEquiv {A B} (f : A -> B)
+  := Build_IsEquiv : forall b, Contr { a : A | f a = b }.
+
+Record Equiv A B
+  := { equiv_fun : A -> B;
+       equiv_isequiv : IsEquiv equiv_fun }.
+
+Arguments equiv_fun {A B} _ _.
+Arguments equiv_isequiv {A B} _ _.
+
+(** Let us use an object of type [Equiv] as a function: *)
+
+Coercion equiv_fun : Equiv >-> Funclass.
+
+(** Tell Coq that the function associated to an [Equiv] object is
+    always an equivalence. *)
+
+Existing Instance equiv_isequiv.
+
+Notation "A <~> B" := (Equiv A B) (at level 70).
+Notation "A ≃ B" := (Equiv A B) (at level 70).
+
+(** We can prove that an equivalence gives us an isomorphism very
+    easily. *)
+
+Definition iso_of_equiv : forall {A B}, A ≃ B -> A ≅ B.
+Proof.
+  refine (fun A B e
+          => {| iso_fun x := e x;
+                iso_isiso := {| iso_inv x := (@center _ (equiv_isequiv e x)).1 |} |}).
+  { intro x.
+    apply (center {a : A | e a = x}).2. }
+  { intro x.
+    refine (@trans _ _ (x; _).1 _ _ _).
+    { apply ap.
+      apply contr. }
+    { exact (refl (x; refl).1). } }
+Defined.
+
+(** We can go the other way with more work. *)
+
+(** Optional Homework: Complete this proof. *)
+
+Definition equiv_of_iso : forall {A B}, A ≅ B -> A ≃ B.
+Proof.
+  refine (fun A B e
+          => {| equiv_fun := e;
+                equiv_isequiv b := {| center := exist (fun a => e a = b) (iso_inv e b) (right_inv e b);
+                                      contr := _ |} |}).
+  intros [a p].
+  destruct p; simpl.
+  apply sigma_decode.
+  pose (q := (trans (ap (iso_inv e) (ap e (sym (left_inv e a))))
+                (trans (ap (iso_inv e) (right_inv e (e a)))
+                       (left_inv e a)))).
+  exists q.
+  simpl.
+  transitivity (trans (sym (ap e q)) (right_inv e _)).
+  { generalize (right_inv e (e a)).
+    clearbody q.
+    revert q.
+    generalize (iso_inv e).
+    intro g.
+    generalize (g (e a)).
+    intros ? q.
+    destruct q; simpl.
+    intro e0; case e0.
+    reflexivity. }
+  { subst q.
+    repeat rewrite <- ?ap_sym, ?sym_trans, ?ap_trans, ?sym_sym, ?trans_pp_p.
+    rewrite !(ap_compose (iso_inv e) e).
+    rewrite (@concat_A1p _ (fun x => e (iso_inv e x)) (right_inv e)).
+    erewrite <- (trans_Vp (ap e left_inv)).
+    rewrite ap_sym.
+    apply ap.
+    rewrite <- !trans_pp_p.
+    rewrite (@concat_A1p _ (fun x => e (iso_inv e x)) (right_inv e)).
+    rewrite trans_pV, trans_1p; reflexivity. }
+Defined.
+
+(** Now, we prove the following helper lemma, which lets us get the
+    right codes for [Equiv].  We again assume functional
+    extensionality. *)
+
+Section assume_funext'.
+  Context (function_decode : forall {A B} {f g : forall a : A, B a}, function_code f g -> f = g)
+          (function_endecode : forall {A B} {f g : forall a : A, B a} (p : function_code f g),
+                                 function_encode (function_decode p) = p)
+          (function_deencode : forall {A B} {f g : forall a : A, B a} (p : f = g),
+                                 function_decode (function_encode p) = p).
+
+  Definition allpath_contr : forall {A} (x y : Contr A), x = y.
+  Proof.
+    intros A x y.
+    destruct x as [x p], y as [y q].
+    cut ((x; p) = (y; q) :> { center : A | forall y, center = y }).
+    { intro H.
+      apply sigma_encode in H.
+      destruct H as [H0 H1]; simpl in *.
+      destruct H0.
+      destruct H1; simpl.
+      reflexivity. }
+    { apply sigma_decode.
+      exists (trans (p y) (q y)).
+      simpl.
+      apply function_decode; intro a.
+      cut (forall p q : y = a, p = q).
+      { intro H; apply H. }
+      { intros p0 q0.
+        refine (trans (sym _) _).
+        { refine (@prop_deencode A (fun x y => trans (sym (p x)) (p y)) _ _ p0). }
+        { refine (@prop_deencode A (fun x y => trans (sym (p x)) (p y)) _ _ q0). } } }
+  Defined.
+
+  Definition allpath_isequiv : forall {A B} (f : A -> B) (e1 e2 : IsEquiv f), e1 = e2.
+  Proof.
+    intros A B f e1 e2.
+    apply function_decode; intro a.
+    apply allpath_contr.
+  Defined.
+
+  Definition equiv_code : forall {A B} (f g : A ≃ B), Type
+    := admit.
+
+  Definition equiv_encode : forall {A B} {f g : A ≃ B}, f = g -> equiv_code f g
+    := admit.
+
+  Definition equiv_decode : forall {A B} {f g : A ≃ B}, equiv_code f g -> f = g
+    := admit.
+
+  Definition equiv_endecode : forall {A B} {f g : A ≃ B} (p : equiv_code f g),
+                              equiv_encode (equiv_decode p) = p
+    := admit.
+
+  Definition equiv_deencode : forall {A B} {f g : A ≃ B} (p : f = g),
+                              equiv_decode (equiv_encode p) = p
+    := admit.
+End assume_funext'.
+
+(** Now that we have a "good" type of isomorphism/equivalence (one
+    with the right equality type), we can go back to the question of
+    [Isomorphic_ap]; Recall that we want to prove:
+
+<<
+Definition Isomorphic_ap : forall (f : Type -> Type) {A B}, A ≅ B -> f A ≅ f B.
+>> *)
+
+(** We can prove this by axiomatizing the codes for types: *)
+
+Definition Type_code' : forall (x y : Type), Type
+  := fun x y => x ≃ y.
+
+Definition Type_encode' : forall {x y : Type}, x = y -> Type_code' x y
+  := admit.
+
+(** The following are unprovable in Coq, currently.  They are
+    collectively known as the "univalence axiom". *)
+
+Axiom Type_decode' : forall {x y : Type}, Type_code' x y -> x = y.
+Axiom Type_endecode' : forall {x y : Type} (p : Type_code' x y),
+                         Type_encode' (Type_decode' p) = p.
+Axiom Type_deencode' : forall {x y : Type} (p : x = y),
+                         Type_decode' (Type_encode' p) = p.
+
+Definition Univalence : forall {x y : Type}, IsEquiv (@Type_encode' x y)
+  := fun x y
+     => equiv_isequiv
+          (equiv_of_iso
+             {| iso_fun := @Type_encode' x y;
+                iso_isiso := {| iso_inv := @Type_decode' x y;
+                                right_inv := Type_endecode';
+                                left_inv := Type_deencode' |} |}).
+
+(** *** Homework: Playing with univalence *)
+
+(** Using univalence, we can prove some things. *)
+
+Definition Empty_set_eq : (Empty_set = Empty_set) = unit :> Type
+  := admit.
+
+Definition unit_eq : (unit = unit) = unit :> Type
+  := admit.
+
+Definition bool_eq : (bool = bool) = bool :> Type
+  := admit.
+
+Definition bool_arrow_bool_eq : (bool -> bool) = (bool * bool)%type
+  := admit.
+
+Definition prod_commutes : forall (A B : Type), (A * B = B * A)%type
+  := admit.
+
+(** Challenge: Show, without axioms, that univalence implies
+    functional extensionality: *)
+
+Definition univalence_implies_funext
+: (forall A B, IsEquiv (@Type_encode' A B))
+  -> (forall A B (f g : forall a : A, B a), (forall a, f a = g a) -> f = g)
+  := admit.
+
+(** Exercise 2.17 from the HoTT Book:
+
+  Show that if [A ≃ A'] and [B ≃ B'], then [(A * B) ≃ (A' * B')] in
+  two ways: once using univalence, and once without assuming it. *)
+
+Definition equiv_functor_prod_univalence
+: (forall A B, IsEquiv (@Type_encode A B))
+  -> forall A A' B B',
+       A ≃ A' -> B ≃ B' -> (A * B ≃ A' * B')%type
+  := admit.
+
+Definition equiv_functor_prod_no_univalence
+: forall A A' B B',
+    A ≃ A' -> B ≃ B' -> (A * B ≃ A' * B')%type
+  := admit.
+
+(** Now prove that these two ways are equal *)
+
+Definition equiv_functor_prod_eq
+: forall univalence,
+    equiv_functor_prod_univalence univalence = equiv_functor_prod_no_univalence
+  := admit.
